More.

theories/common/treemap.v
@@ -6,35 +6,55 @@ From zoo Require Import
 From zoo Require Import
   options.
 
-Definition treemap N `{Countable N} E :=
-  gmap N (N * E).
-
 Section treemap_rooted.
   Context {N} `{Countable N} {E : Type}.
 
   Implicit Types node root src dst : N.
   Implicit Types edge : E.
-  Implicit Types edges : list E.
+  Implicit Types path : list E.
   Implicit Types ϵ : N * E.
-  Implicit Types tree : treemap N E.
+  Implicit Types tree : gmap N (N * E).
 
-  Inductive treemap_path tree root : N → list E → Prop :=
+  Inductive treemap_path tree dst : N → list E → Prop :=
     | treemap_path_nil :
-        treemap_path tree root root []
-    | treemap_path_cons {node1} ϵ node2 edge edges :
+        treemap_path tree dst dst []
+    | treemap_path_cons {node1} ϵ node2 edge path :
         tree !! node1 = Some ϵ →
         ϵ.1 = node2 →
         ϵ.2 = edge →
-        treemap_path tree root node2 edges →
-        treemap_path tree root node1 (edge :: edges).
+        treemap_path tree dst node2 path →
+        treemap_path tree dst node1 (edge :: path).
   #[local] Hint Constructors treemap_path : core.
 
   Definition treemap_rooted tree root :=
     tree !! root = None ∧
       ∀ node,
       is_Some (tree !! node) →
-        ∃ edges,
-        treemap_path tree root node edges.
+        ∃ path,
+        treemap_path tree root node path.
+
+  Definition treemap_reroot tree root root' edge:=
+    <[root := (root', edge)]> (delete root' tree).
+
+  Lemma treemap_path_app tree dst1 node path1 dst2 path2 :
+    treemap_path tree dst1 node path1 →
+    treemap_path tree dst2 dst1 path2 →
+    treemap_path tree dst2 node (path1 ++ path2).
+  Proof.
+    induction 1; naive_solver.
+  Qed.
+
+  Lemma treemap_path_mono {tree dst node path} tree' :
+    tree ##ₘ tree' →
+    treemap_path tree dst node path →
+    treemap_path (tree ∪ tree') dst node path.
+  Proof.
+    intros Htree'. induction 1; first done.
+    econstructor; [| done..].
+    rewrite lookup_union_l //.
+    apply eq_None_ne_Some_2 => ? ?.
+    rewrite map_disjoint_spec in Htree'. naive_solver.
+  Qed.
 
   Lemma treemap_rooted_empty root :
     treemap_rooted ∅ root.
@@ -43,39 +63,122 @@ Section treemap_rooted.
     intros node []%(lookup_empty_is_Some (A := N * E)).
   Qed.
 
-  Axiom treemap_rooted_lift : ∀ {tree root} root_edge root',
+  Lemma treemap_path_is_nil tree root path :
     treemap_rooted tree root →
-    tree !! root' = None →
-    treemap_rooted (<[root := (root', root_edge)]> tree) root'.
-
-  Lemma treemap_rooted_path {tree root} node :
-    treemap_rooted tree root →
-    is_Some (tree !! node) →
-      ∃ edges,
-      treemap_path tree root node edges.
-  Proof.
-    rewrite /treemap_rooted. naive_solver.
-  Qed.
-
-  Lemma treemap_path_is_nil tree root edges :
-    treemap_rooted tree root →
-    treemap_path tree root root edges →
-    edges = [].
+    treemap_path tree root root path →
+    path = [].
   Proof.
     intros (Hlookup_root & _) Hpath.
     invert Hpath. done.
   Qed.
-  Lemma treemap_path_is_cons tree root node edges :
+  Lemma treemap_path_is_cons tree root node path :
     treemap_rooted tree root →
-    treemap_path tree root node edges →
+    treemap_path tree root node path →
     node ≠ root →
-      ∃ node' edge edges',
-      edges = edge :: edges' ∧
+      ∃ node' edge path',
+      path = edge :: path' ∧
       tree !! node = Some (node', edge) ∧
-      treemap_path tree root node' edges'.
+      treemap_path tree root node' path'.
   Proof.
     intros Hrooted Hpath Hnode.
     invert Hpath as [| ? []]. naive_solver.
+  Qed.
+
+  #[local] Lemma treemap_path_acyclic {tree root path} node ϵ :
+    treemap_rooted tree root →
+    treemap_path tree root node path →
+    tree !! node = Some ϵ →
+    ϵ.1 ≠ node.
+  Proof.
+    rewrite /treemap_rooted. induction 2; naive_solver.
+  Qed.
+  Lemma treemap_rooted_acyclic {tree root} node ϵ :
+    treemap_rooted tree root →
+    tree !! node = Some ϵ →
+    ϵ.1 ≠ node.
+  Proof.
+    intros (Hlookup_root & Hrooted) Hlookup.
+    odestruct Hrooted as (path & Hpath); first done.
+    eapply treemap_path_acyclic; done.
+  Qed.
+
+  Lemma treemap_rooted_path {tree root} node :
+    treemap_rooted tree root →
+    is_Some (tree !! node) →
+      ∃ path,
+      treemap_path tree root node path.
+  Proof.
+    rewrite /treemap_rooted. naive_solver.
+  Qed.
+
+  Lemma treemap_rooted_lift {tree root} root' edge :
+    treemap_rooted tree root →
+    tree !! root' = None →
+    root ≠ root' →
+    treemap_rooted (<[root := (root', edge)]> tree) root'.
+  Proof.
+    set tree' := <[root := (root', edge)]> tree.
+    intros (Htree_lookup_root & Hrooted) Htree_lookup_root' Hroot'. split.
+    - rewrite lookup_insert_ne //.
+    - intros node (ϵ & Htree'_lookup_node).
+      assert (tree' !! root = Some (root', edge)) as Htree'_lookup_root.
+      { rewrite lookup_insert //. }
+      assert (treemap_path tree' root' root [edge]) as Hpath_root.
+      { econstructor; done. }
+      destruct (decide (node = root)) as [-> | Hnode]; first eauto.
+      pose proof Htree'_lookup_node as Htree_lookup_node.
+      rewrite lookup_insert_ne // in Htree_lookup_node.
+      odestruct Hrooted as (path & Hpath); first done.
+      exists (path ++ [edge]). eapply treemap_path_app; last done.
+      rewrite /tree' insert_union_singleton_r //.
+      apply treemap_path_mono; last done.
+      solve_map_disjoint.
+  Qed.
+
+  Lemma treemap_reroot_path {tree root} root' ϵ edge node path :
+    treemap_rooted tree root →
+    tree !! root' = Some ϵ →
+    ϵ.1 = root →
+    treemap_path tree root' node path →
+    treemap_path (treemap_reroot tree root root' edge) root' node path.
+  Proof.
+    set tree' := treemap_reroot tree root root' edge.
+    destruct ϵ as (_root, edge').
+    intros (Htree_lookup_root & Hrooted) Htree_lookup_root' [= ->].
+    assert (root ≠ root') as Hroot' by congruence.
+    induction 1 as [| node ϵ node' edge'' path Htree_lookup_node ? ? Hpath Hpath']; first done.
+    destruct (decide (node = root)) as [-> | Hnode]; first congruence.
+    destruct (decide (node = root')) as [-> | Hnode_]; first invert Hpath.
+    econstructor; try done.
+    rewrite lookup_insert_ne // lookup_delete_ne //.
+  Qed.
+  Lemma treemap_reroot_rooted {tree root} root' ϵ edge :
+    treemap_rooted tree root →
+    tree !! root' = Some ϵ →
+    ϵ.1 = root →
+    treemap_rooted (treemap_reroot tree root root' edge) root'.
+  Proof.
+    set tree' := treemap_reroot tree root root' edge.
+    destruct ϵ as (_root, edge').
+    intros (Htree_lookup_root & Hrooted) Htree_lookup_root' [= ->].
+    assert (root ≠ root') as Hroot' by congruence.
+    split.
+    - rewrite lookup_insert_ne // lookup_delete //.
+    - intros node (ϵ & Htree'_lookup_node).
+      assert (tree' !! root = Some (root', edge)) as Htree'_lookup_root.
+      { rewrite lookup_insert //. }
+      assert (treemap_path tree' root' root [edge]) as Hpath_root.
+      { econstructor; done. }
+      destruct (decide (node = root)) as [-> | Hnode]; first eauto.
+      rewrite lookup_insert_ne // in Htree'_lookup_node.
+      apply lookup_delete_Some in Htree'_lookup_node as (Hnode_ & Htree_lookup_node).
+      odestruct Hrooted as (path & Hpath); first done.
+      clear- Htree_lookup_root Hpath_root Hpath.
+      induction Hpath as [| node ϵ node' edge' path Htree_lookup_node ? ? Hpath (path' & Hpath')]; first eauto.
+      destruct (decide (node = root')) as [-> | Hnode]; first eauto.
+      exists (edge' :: path'). econstructor; try done.
+      rewrite lookup_insert_ne; first congruence.
+      rewrite lookup_delete_ne //.
   Qed.
 End treemap_rooted.
 
